\documentclass{article}
\usepackage[margin=1.0in]{geometry}
\usepackage{amssymb}
\usepackage{amsmath}
\usepackage{enumitem}
\usepackage{mathtools}
\usepackage{bm}
\usepackage{graphicx}
\begin{document}


\begin{center}
Econometrics Assignment 5 \\
Eric Tu
\end{center}

	$Pr[resp_{i} = 1] = \cfrac{exp(\beta_{0} + \beta_{1} male_{i} + \beta_{2} active_{i} + \beta_{3} age_{i} + \beta_{4}(age_{i}/10)^{2})}{1+exp(\beta_{0} + \beta_{1} male_{i} + \beta_{2} active_{i} + \beta_{3} age_{i} + \beta_{4}(age_{i}/10)^{2})}$ 

	$\begin{matrix}
	Variable & Coefficient \\
	Intercept & -2.488 \\
	Male & 0.954 \\
	Active & 0.914 \\
	Age & 0.070 \\
	(Age/10)^{2} & -0.069 \\
	\end{matrix}$

\begin{enumerate}[label=(\alph*)]

	\item{}
	For a 50 year old active male customer
	\begin{center}
	$Pr[resp_{i} = 0]active_{i} \beta_{2}$ \\ [4pt]
	$ (1 - Pr[resp_{i} =1])active_{i} \beta_{2}$ \\ [4pt]
	$ \cfrac{1}{1+exp(-2.488 + 0.954 + 0.914 + 0.070 * 50 -0.069 * 25)} (0.914 * 1) $ \\[4pt]
	$ = 0.229 $ \\ [4pt]
	\end{center}
	
	For a 50 year old inactive male customer \\
	\begin{center}
	$\cfrac{1}{1+exp(-2.488 + 0.954 + 0.070 * 50 -0.069 * 25)} (0.914 * 0) $ \\
	$= 0$ \\
	\end{center}
	
	\item
	Let $Z =  exp(\beta_{0} + \beta_{1} male_{i} + \beta_{3} age_{i} + \beta_{4}(age_{i}/10)^{2}) $\\ [6pt]
	then $exp(\beta_{2})Z = exp(\beta_{0} + \beta_{1} male_{i} + \beta_{2} + \beta_{3} age_{i} + \beta_{4}(age_{i}/10)^{2})$ \\ [6pt]
	
	\begin{center}
	$\cfrac{Pr[resp_{i}=1|active_{i}=1] - Pr[resp_{i}=1|active_{i}=0]}{Pr[resp_{i}=1|active_{i}=0]}	$ \\ [6pt]
	$\cfrac{\cfrac{exp(\beta_{2})Z}{1 + Zexp(\beta_{2})} - \cfrac{Z}{1+Z}}{\cfrac{Z}{1+Z}}$ \\	[6pt]
	$(\cfrac{1+Z}{Z})\cfrac{exp(\beta_{2})Z}{1 + Zexp(\beta_{2})} - (\cfrac{1+Z}{Z})\cfrac{Z}{1+Z}$ \\ [6pt]
	$ \cfrac{(1+Z)exp(\beta_{2})}{1 + Zexp(\beta_{2})} - 1$ \\ [6pt]
	$ \cfrac{Zexp(\beta_{2}) + exp(\beta_{2}) - 1 - Zexp(\beta_{2})}{1 + Zexp(\beta_{2})}$ \\ [6pt]
	$ \cfrac{exp(\beta_{2}) - 1}{1 + Zexp(\beta_{2})}$ \\ [6pt]
	$ (exp(\beta_{2}) - 1)\cfrac{1}{1 + Zexp(\beta_{2})}$ \\ [6pt]
	\end{center}
	\textit{Using $Pr[resp_{i}=0|active_{i}=1] = 1 - Pr[resp_{i}=1|active_{i}] = \cfrac{1}{1 + Zexp(\beta_{2})}$} \\ [6pt]
	\begin{center}
	$ (exp(\beta_{2}) - 1)Pr[resp_{i}=0|active_{i}=1] $ \\	[6pt]
	\end{center}

		
	
	\item
	$(exp(\beta_{2}) - 1) Pr[ resp_{i} =0 | active_{i} =1]$ \\[4pt]
	\begin{center}
	$(exp(0.914) -1) \cfrac{1}{1+exp(-2.488 + 0.954 + 0.914 + 0.070 * 50 -0.069 * 25)}$ \\[4pt]
	$ = 0.365$ \\ [8pt]
	\end{center}
\end{enumerate}

\end{document}
